02Stack/Stack.thy
@@ -30,4 +30,16 @@ primrec devalue :: "val \<Rightarrow> expr" where
 | "devalue (VFold t x) = Fold t x"
 | "devalue (VTyAbs k e) = TyAbs k e"
 
+primrec free_vars\<^sub>s :: "frame \<Rightarrow> nat set" where
+  "free_vars\<^sub>s (SRef x) = {x}"
+| "free_vars\<^sub>s (SApp e) = free_vars e"
+| "free_vars\<^sub>s (SProj l) = {}"
+| "free_vars\<^sub>s (SCase t cs) = free_vars\<^sub>c cs"
+| "free_vars\<^sub>s (SUnfold t) = {}"
+| "free_vars\<^sub>s (STyApp t) = {}"
+
+primrec free_vars\<^sub>s\<^sub>s :: "frame list \<Rightarrow> nat set" where
+  "free_vars\<^sub>s\<^sub>s [] = {}"
+| "free_vars\<^sub>s\<^sub>s (f # s) = free_vars\<^sub>s f \<union> free_vars\<^sub>s\<^sub>s s"
+
 end
