02Stack/StackCorrectness.thy
@@ -2,39 +2,54 @@ theory StackCorrectness
 imports "EvaluateStack" "../01Expression/Evaluate" "../Utilities/Iterate"
 begin
 
-inductive unstack :: "frame list \<Rightarrow> expr \<Rightarrow> expr heap \<Rightarrow> frame list \<Rightarrow> expr \<Rightarrow> expr heap \<Rightarrow> bool" where
-  us_nil [simp]: "unstack [] e h [] e h"
-| us_sref [simp]: "unstack s (Var x) (update\<^sub>h h x e) s' e' h' \<Longrightarrow> unstack (SRef x # s) e h s' e' h'"
-| us_sapp [simp]: "unstack s (App e e\<^sub>2) h s' e' h' \<Longrightarrow> unstack (SApp e\<^sub>2 # s) e h s' e' h'"
-| us_sproj [simp]: "unstack s (Proj e l) h s' e' h' \<Longrightarrow> unstack (SProj l # s) e h s' e' h'"
-| us_scase [simp]: "unstack s (Case e t cs) h s' e' h' \<Longrightarrow> unstack (SCase t cs # s) e h s' e' h'"
-| us_sunfold [simp]: "unstack s (Unfold t e) h s' e' h' \<Longrightarrow> unstack (SUnfold t # s) e h s' e' h'"
-| us_styapp [simp]: "unstack s (TyApp e t) h s' e' h' \<Longrightarrow> unstack (STyApp t # s) e h s' e' h'"
-| us_let [simp]: "length\<^sub>h h > 0 \<Longrightarrow> unextend\<^sub>h h = (e', h') \<Longrightarrow> 
-    unstack s (Let e' e) h' s'' e'' h'' \<Longrightarrow> unstack s e h s'' e'' h''"
+inductive unstack :: "nat set \<Rightarrow> frame list \<Rightarrow> expr \<Rightarrow> expr heap \<Rightarrow> nat set \<Rightarrow> frame list \<Rightarrow> expr \<Rightarrow> 
+    bool" where
+  us_nil [simp]: "unstack xs [] e h xs [] e"
+| us_sref [simp]: "unstack xs s (Var x) (update\<^sub>h h x e) xs' s' e' \<Longrightarrow> 
+    unstack xs (SRef x # s) e h xs' s' e'"
+| us_sapp [simp]: "unstack xs s (App e e\<^sub>2) h xs' s' e' \<Longrightarrow> unstack xs (SApp e\<^sub>2 # s) e h xs' s' e'"
+| us_sproj [simp]: "unstack xs s (Proj e l) h xs' s' e' \<Longrightarrow> unstack xs (SProj l # s) e h xs' s' e'"
+| us_scase [simp]: "unstack xs s (Case e t cs) h xs' s' e' \<Longrightarrow> 
+    unstack xs (SCase t cs # s) e h xs' s' e'"
+| us_sunfold [simp]: "unstack xs s (Unfold t e) h xs' s' e' \<Longrightarrow> 
+    unstack xs (SUnfold t # s) e h xs' s' e'"
+| us_styapp [simp]: "unstack xs s (TyApp e t) h xs' s' e' \<Longrightarrow> unstack xs (STyApp t # s) e h xs' s' e'"
+| us_let [simp]: "x \<notin> free_vars\<^sub>s\<^sub>s s \<Longrightarrow> x \<notin> xs \<Longrightarrow>
+    unstack (insert x xs) s (Let (lookup\<^sub>h x h) (incr\<^sub>e\<^sub>e x (subst\<^sub>x\<^sub>e x 0 e))) h xs' s' e' \<Longrightarrow> 
+      unstack xs s e h xs' s' e'"
 
 inductive unstack_state :: "stack_state \<Rightarrow> expr \<Rightarrow> bool" where
-  uss_eval [simp]: "unstack s e h [] e' empty\<^sub>h \<Longrightarrow> unstack_state (StackState (Eval e) s h) e'"
-| uss_return [simp]: "unstack s (devalue v) h [] e' empty\<^sub>h \<Longrightarrow> 
+  uss_eval [simp]: "unstack {} s e h (zero_to (length\<^sub>h h)) [] e' \<Longrightarrow> 
+    unstack_state (StackState (Eval e) s h) e'"
+| uss_return [simp]: "unstack {} s (devalue v) h (zero_to (length\<^sub>h h)) [] e' \<Longrightarrow> 
     unstack_state (StackState (Return v) s h) e'"
 
-lemma tc_unstack [elim]: "unstack s e h [] e' empty\<^sub>h \<Longrightarrow> \<Gamma> \<turnstile>\<^sub>s\<^sub>s s : t \<rightarrow> t' \<Longrightarrow> [],\<Gamma> \<turnstile> e : t \<Longrightarrow> 
-    h \<turnstile>\<^sub>h \<Gamma> \<Longrightarrow> [],[] \<turnstile> e' : t'"
-  proof (induction s e h "[] :: frame list" e' "empty\<^sub>h :: expr heap" arbitrary: \<Gamma> t 
+lemma tc_unstack [elim]: "unstack xs s e h (zero_to (length \<Gamma>)) [] e' \<Longrightarrow> \<Gamma> \<turnstile>\<^sub>s\<^sub>s s : t \<rightarrow> t' \<Longrightarrow> 
+  [],\<Gamma> \<turnstile> e : t \<Longrightarrow> h \<turnstile>\<^sub>h \<Gamma> \<Longrightarrow> free_vars e \<inter> xs = {} \<Longrightarrow> free_vars\<^sub>s\<^sub>s s \<inter> xs = {} \<Longrightarrow> 
+    (\<forall>x \<in> xs. \<forall>x \<in> zero_to (length \<Gamma>). y \<notin> xs \<longrightarrow> x \<notin> free_vars (lookup\<^sub>h y h)) \<Longrightarrow> [],[] \<turnstile> e' : t'"
+  proof (induction xs s e h "(zero_to (length \<Gamma>))" "[] :: frame list" e' arbitrary: \<Gamma> t 
          rule: unstack.induct)
-  case (us_let h e' h' s e e'')
-    from us_let have "unextend\<^sub>h h = (e', h')" by simp
-    from us_let have "unstack s (Let e' e) h' [] e'' empty\<^sub>h" by simp
-    from us_let have "x\<Gamma> \<turnstile>\<^sub>s\<^sub>s s : xt \<rightarrow> t' \<Longrightarrow> [] ,x\<Gamma> \<turnstile> expr.Let e' e : xt \<Longrightarrow> h' \<turnstile>\<^sub>h x\<Gamma> \<Longrightarrow> [],[] \<turnstile> e'' : t'" by simp
-    from us_let have "\<Gamma> \<turnstile>\<^sub>s\<^sub>s s : t \<rightarrow> t'" by simp
-    from us_let have "[] ,\<Gamma> \<turnstile> e : t" by simp
-    from us_let have "h \<turnstile>\<^sub>h \<Gamma>" by simp
+  case (us_nil e h)
+    thus ?case by simp
+  next case us_sref
+    thus ?case by simp
+  next case us_sapp
+    thus ?case by simp
+  next case us_sproj
+    thus ?case by simp
+  next case us_scase
+    thus ?case by simp
+  next case us_sunfold
+    thus ?case by simp
+  next case us_styapp
+    thus ?case by simp
+  next case (us_let x s xs h e e')
 
 
 
-    have "[],[] \<turnstile> e'' : t'" by simp
-    thus ?case by fastforce
-  qed fastforce+
+    have "[],[] \<turnstile> e' : t'" by simp
+    thus ?case by simp
+  qed
 
 lemma tc_unstack_state [elim]: "unstack_state \<Sigma> e \<Longrightarrow> \<Sigma> hastype t \<Longrightarrow> [],[] \<turnstile> e : t"
   proof (induction \<Sigma> e rule: unstack_state.induct)
